also hiding res now

misc-verification/slab_allocator.v
@@ -53,39 +53,34 @@ Section Hoare.
   Implicit Types n i res cap size : nat.
   Implicit Types v w : val.
 
-  Definition is_valid_loc l al res : iProp Σ := 
-    ∃ (i : nat), ⌜l = (al +ₗ (3 + i))⌝ ∗ ⌜i < res⌝.
-  (*TODO: add exists res box*)
-  (*
-     ⌜(al +ₗ 3) ≤ₗ l⌝ ∗ ⌜l <ₗ (al +ₗ (3 + res))⌝. *)
+  Definition is_valid_loc l al : iProp Σ := 
+    ∃ res (i : nat), (al +ₗ 1) ↦□ #res ∗ ⌜l = (al +ₗ (3 + i))⌝ ∗ ⌜i < res⌝.
 
-  Global Instance is_valid_loc_presist l al res : Persistent (is_valid_loc l al res).
+  Global Instance is_valid_loc_presist l al : Persistent (is_valid_loc l al).
   Proof. apply _. Qed.
 
-  Fixpoint is_freelist_rec l al res size : iProp Σ := 
+  Fixpoint is_freelist_rec l al size : iProp Σ := 
     match size with 
-    | O => l ↦ NONEV ∗ is_valid_loc l al res 
-    | S s => ∃ l1, l ↦ SOMEV #l1 ∗ is_valid_loc l al res ∗ is_freelist_rec l1 al res s
+    | O => l ↦ NONEV ∗ is_valid_loc l al 
+    | S s => ∃ l1, l ↦ SOMEV #l1 ∗ is_valid_loc l al ∗ is_freelist_rec l1 al s
     end.
     
-  Definition is_freelist l al res : iProp Σ := 
+  Definition is_freelist l al : iProp Σ := 
     l ↦ NONEV 
       ∨
-    (*is size here going to work, i guess we only need size for is_freelist rec?
-       and then it really means amound allocated - 1?*)
-    ∃ l1 size, l ↦ SOMEV #l1 ∗ (*⌜size ≤ cap⌝ ∗ does not work in freelists_push
-                                      _hoare otherwise..*) 
-    is_freelist_rec l1 al res size.
+    ∃ l1 size, l ↦ SOMEV #l1 ∗ is_freelist_rec l1 al size.
 
-  Definition is_allocator (l : loc) (res : nat) : iProp Σ := 
-    ∃ cap vs, ⌜res > 0⌝ ∗ ⌜cap ≤ res⌝ ∗ (l +ₗ 1) ↦ #res ∗ 
-      (l +ₗ 2) ↦ #cap ∗ is_freelist l l res ∗  (*TODO: add res box*)
-      (l +ₗ (3 + cap)) ↦∗ vs ∗ ⌜length vs = res - cap⌝.
+  (*res now has fractional ownership and is only readable (box) 
+    now we can hide it, now can also never free l +ₗ 1*)
+  Definition is_allocator (al : loc) : iProp Σ := 
+    ∃ res cap vs, ⌜res > 0⌝ ∗ ⌜cap ≤ res⌝ ∗ (al +ₗ 1) ↦□  #res ∗ 
+      (al +ₗ 2) ↦ #cap ∗ is_freelist al al ∗  
+      (al +ₗ (3 + cap)) ↦∗ vs ∗ ⌜length vs = res - cap⌝.
 
-  Lemma new_alloc_hoare l res : 
+  Lemma new_alloc_hoare res : 
     {{{ ⌜res > 0⌝ }}} 
       new_alloc_lazy #res 
-    {{{ l, RET #l; is_allocator l res }}}.
+    {{{ al, RET #al; is_allocator al }}}.
   Proof. 
     iIntros (φ) "%Hn Hphi". iUnfold new_alloc_lazy. wp_pures.
     wp_apply wp_allocN; [lia|done|]. iIntros "%al (HalN & _)". 
@@ -93,51 +88,57 @@ Section Hoare.
     rewrite Heq. simpl. rewrite 3!array_cons.
     iDestruct "HalN" as "(Hal & Hal1 & Hal2 & HalN)". wp_store. wp_store. 
     rewrite 2!Loc.add_assoc. wp_store. iApply "Hphi". 
-    iUnfold is_allocator. iExists 0. iFrame. 
-    iSplitR; [by iPureIntro|]. iSplitR; [iPureIntro; lia|].
+    iExists res, 0. iMod (pointsto_persist with "Hal1") as "#Hal1". iFrame.
+    iSplitR; [by iPureIntro|]. iSplitR; [iPureIntro; lia|]. iSplitR; [done|].
     iPureIntro. rewrite length_replicate. lia.
   Qed.
 
-   Lemma freelist_pop_hoare fl al res : 
-    {{{ is_freelist fl al res }}} 
+   Lemma freelist_pop_hoare fl al : 
+    {{{ is_freelist fl al }}} 
       freelist_pop #fl
     {{{ vret, RET vret; 
-      ⌜vret = NONEV⌝ ∗ is_freelist fl al res 
+      is_freelist fl al ∗
+      (⌜vret = NONEV⌝ 
         ∨ 
-      ∃ l v, ⌜vret = SOMEV #l⌝ ∗ l ↦ v ∗ is_valid_loc l al res ∗ is_freelist fl al res 
+      ∃ l v, ⌜vret = SOMEV #l⌝ ∗ l ↦ v ∗ is_valid_loc l al)
     }}}. 
   Proof.
     iIntros (φ) "[Hl | (%l1 & %s & Hl & Hflr)] Hphi"; 
     iUnfold freelist_pop; wp_load; wp_pures.
-    { iApply "Hphi". iLeft. by iFrame. }
+    { iApply "Hphi". iFrame. by iLeft. }
     destruct s; simpl.
     { iDestruct "Hflr" as "(Hl1 & Hvl)". wp_load. wp_store. wp_pures. 
-      iApply "Hphi". iRight. by iFrame. }
+      iApply "Hphi". iFrame. iRight. by iFrame. }
     iDestruct "Hflr" as "(%l0 & Hl1 & Hl1v & Hflr)". wp_load. wp_store.
-    wp_pures. iApply "Hphi". iRight. iUnfold is_freelist. iFrame.
-    iSplitR; [by iPureIntro|]. iRight. iFrame. iPureIntro. lia.
+    wp_pures. iApply "Hphi". iSplitR "Hl1 Hl1v"; [iRight; by iFrame|].
+    iRight. by iFrame.   
   Qed.
 
-  Lemma freelist_push_hoare l fl al res : 
-    {{{ is_freelist fl al res ∗ (∃ v, l ↦ v) ∗ is_valid_loc l al res }}}
+  Lemma freelist_push_hoare l fl al : 
+    {{{ is_freelist fl al ∗ (∃ v, l ↦ v) ∗ is_valid_loc l al }}}
       freelist_push #fl #l
-    {{{ RET #(); is_freelist fl al res }}}.
+    {{{ RET #(); is_freelist fl al }}}.
   Proof. 
     iIntros (φ) "([Hfl|(%l1&%s&Hfl&Hisfl)]&(%v&Hl)&Hlv) Hphi"; 
     iUnfold freelist_push; wp_load; wp_store; wp_store.
-    { iApply "Hphi". iRight. iFrame. iExists 0. (*iSplitR; [iPureIntro; lia|]. *)
-      iUnfold is_freelist_rec. by iFrame. }
+    { iApply "Hphi". iRight. iFrame. iExists 0. by iFrame. }
     iApply "Hphi". iRight. iExists l, (S s). by iFrame. 
   Qed.
 
-  Lemma free_hoare l al res : 
-    {{{ is_allocator al res ∗ (∃ v, l ↦ v) ∗ is_valid_loc l al res }}}
+  (*shouldn't we have a problem here? 
+     since we own a lot of locations that are valid locations 
+     it is possible that l is one of those locations and then 
+     we should derive a contradiciton..
+     but from alloc you always get an is_valid_loc that is 
+     also within cap so it should not be an issue *)
+  Lemma free_hoare l al : 
+    {{{ is_allocator al ∗ (∃ v, l ↦ v) ∗ is_valid_loc l al }}}
       free #al #l
-    {{{ RET #(); is_allocator al res }}}.
+    {{{ RET #(); is_allocator al }}}.
   Proof.
-    iIntros (φ) "((%cap&%vs&%Hr&%Hcr&Hal1&Hal2&Hfl&Hun) & (%v & Hl) & #Hlv) Hphi".
-    iUnfold free. wp_pures. iApply (freelist_push_hoare with "[Hfl Hl]"); 
-    [by iFrame|]. iNext. iIntros "Hfl". iApply "Hphi". iFrame. auto.
+    iIntros (φ) "((%res&%cap&%vs&%Hr&%Hcr&Hal1&Hal2&Hfl&Hun) & (%v & Hl) & #Hlv) Hphi".
+    iUnfold free. wp_pures. iApply (freelist_push_hoare with "[Hfl Hl]"); [by iFrame|].
+    iNext. iIntros "Hfl". iApply "Hphi". iFrame. auto.
   Qed.
 
   Lemma freelist_extend_hoare fl al res lb cap n c d : 
@@ -145,54 +146,57 @@ Section Hoare.
     lb = (al +ₗ (3 + cap)) ->
     cap ≤ res ->
     n ≤ res - cap ->
-    {{{ is_freelist fl al res ∗ ∃ vs, (lb +ₗ c) ↦∗ vs ∗ ⌜length vs = d⌝ }}} 
+    {{{ 
+      (al +ₗ 1) ↦□ #res ∗ 
+      is_freelist fl al ∗ ∃ vs, (lb +ₗ c) ↦∗ vs ∗ ⌜length vs = d⌝ 
+    }}} 
       freelist_extend #fl #lb #n #c
-    {{{ RET #(); is_freelist fl al res }}}. 
+    {{{ RET #(); is_freelist fl al }}}. 
   Proof. 
     iInduction d as [|d IH] forall (c); simpl; 
-    iIntros (Hd -> Hcr Hd2 φ) "(Hisfl & %vs & Hun & %Hlen) Hphi"; 
+    iIntros (Hd -> Hcr Hd2 φ) "(#Hal1 & Hisfl & %vs & Hun & %Hlen) Hphi"; 
     iUnfold freelist_extend; wp_pures. 
     { case_bool_decide; [lia|]. wp_pures. by iApply "Hphi". }
     case_bool_decide; [|lia]. wp_pures. destruct vs;
     [rewrite length_nil in Hlen; lia|]. rewrite array_cons.
     iDestruct "Hun" as "(Hun1 & Hun)". 
     wp_apply (freelist_push_hoare with "[Hisfl Hun1]").
-    { iFrame. iExists (cap + c). rewrite Loc.add_assoc. iPureIntro.
-      split; [|lia]. by rewrite Nat2Z.inj_add Z.add_assoc. }
+    { iFrame. iExists res, (cap + c). iFrame "Hal1". rewrite Loc.add_assoc. 
+      iPureIntro. split; [|lia]. by rewrite Nat2Z.inj_add Z.add_assoc. }
     iIntros "Hisfl". wp_pure. wp_pure. wp_pure. fold freelist_extend.  
     assert (Heq : (Z.of_nat c + 1)%Z = Z.of_nat (c + 1)) by lia. rewrite Heq. 
     iApply ("IH" with "[] [] [] [] [Hisfl Hun]"); 
     try iPureIntro; [lia|done|lia|lia| |]. 
-    { iSplitR "Hun"; [done|]. iExists vs. iSplitL; 
+    { iFrame "Hal1". iSplitR "Hun"; [done|]. iExists vs. iSplitL; 
       [by rewrite Loc.add_assoc Nat2Z.inj_add|]. iPureIntro. simpl in Hlen. lia. }
     iNext. iIntros "Hfl". by iApply "Hphi".  
   Qed. 
 
-  Lemma extend_hoare al res : 
-    {{{ is_allocator al res }}} 
+  Lemma extend_hoare al : 
+    {{{ is_allocator al }}} 
       extend #al 
-      {{{ vret, RET vret; is_allocator al res ∗ 
-        ((∃ l v, ⌜vret = SOMEV #l⌝ ∗ l ↦ v ∗ is_valid_loc l al res) 
+      {{{ vret, RET vret; 
+        is_allocator al ∗ 
+        ((∃ l v, ⌜vret = SOMEV #l⌝ ∗ l ↦ v ∗ is_valid_loc l al) 
           ∨  
         ⌜vret = NONEV⌝)
       }}}.
   Proof. 
-    iIntros (φ) "(%cap & %vs & %Hr & %Hcr & Hal1 & Hal2 & Hisfl & Hun & %Hlen) Hphi".
+    iIntros (φ) "(%res&%cap&%vs&%Hr&%Hcr & #Hal1 & Hal2 & Hisfl & Hun & %Hlen) Hphi".
     iUnfold extend. wp_pures. wp_load. wp_load. wp_pures. 
     destruct (decide (cap = 0)) as [Hc | Hc]. 
-    (*cap = 0 branch, mext = 1*)
     { rewrite Hc. wp_pures. case_bool_decide; [|lia]. wp_pures. 
       wp_apply ((freelist_extend_hoare al al res (al +ₗ 3) 0 0 0 0) with "[Hisfl]"); 
       try lia; [assert ((3 + Z.of_nat 0)%Z = 3) by lia; by rewrite H0| |].
-      { iSplitL "Hisfl"; [done|]. iExists []. iSplit; [by rewrite array_nil|iPureIntro;
-          by rewrite length_nil]. }
+      { iFrame "Hal1". iSplitL "Hisfl"; [done|]. iExists []. iSplit; 
+        [by rewrite array_nil|iPureIntro; by rewrite length_nil]. }
       destruct vs; [rewrite length_nil in Hlen; lia|]. rewrite array_cons.
       iDestruct "Hun" as "(Hun1 & Hun)".
       iIntros "Hisfl". wp_store. wp_pures. iApply "Hphi". iSplitR "Hun1". 
-      { iUnfold is_allocator. iExists 1, vs. iFrame. iSplitR; [by iPureIntro|].
-        iSplitR; [by iPureIntro|]. iSplitL; [by rewrite Loc.add_assoc|]. 
-        iPureIntro. simpl in Hlen. lia. }
-      iLeft. iExists (al +ₗ 3), v. iFrame. iSplitL; [done|]. iExists 0. auto. }
+      { iExists res, 1, vs. rewrite Loc.add_assoc. iFrame. iFrame "Hal1". 
+        iSplitR; [by iPureIntro|]. iSplitR; [by iPureIntro|]. iPureIntro. 
+        simpl in Hlen. lia. }
+      iLeft. iExists (al +ₗ 3), v. iFrame. iSplitL; [done|]. iExists res, 0. auto. }
     case_bool_decide; [inv H; lia|]. wp_pures. case_bool_decide.
     { wp_pures. case_bool_decide; [inv H1; lia|]. wp_pures. 
       assert (Z.of_nat (cap - 1) = (Z.of_nat cap - 1)%Z) by lia. rewrite -H2.
@@ -201,13 +205,12 @@ Section Hoare.
       assert (Hlt : length (take (cap - 1) vs) = cap - 1); [rewrite length_take; lia|].
       wp_apply (freelist_extend_hoare al al res (al +ₗ (3 + cap)) 
       cap (cap - 1) 0 (cap - 1) with "[Hisfl Hun1]"); try lia; [done| |].
-      { iSplitL "Hisfl"; [done|]. rewrite Loc.add_0. iFrame. 
-        iPureIntro. by rewrite Hlt. }
+      { iFrame "Hal1 Hisfl". rewrite Loc.add_0. iFrame. iPureIntro. by rewrite Hlt. }
       iIntros "Hisfl". wp_store. wp_pures. iApply "Hphi". rewrite Hlt. 
       rewrite -(take_drop 1 (drop (cap - 1) vs)). 
       iDestruct (array_app with "Hun2") as "(Hun1 & Hun2)". iSplitR "Hun1". 
-      { iUnfold is_allocator. iExists (cap + cap), (drop cap vs). 
-        rewrite Nat2Z.inj_add. iFrame. iSplitR; [iPureIntro; lia|]. 
+      { iExists res, (cap + cap), (drop cap vs). rewrite Nat2Z.inj_add. 
+        iFrame. iFrame "Hal1". iSplitR; [iPureIntro; lia|]. 
         iSplitR; [iPureIntro; lia|]. rewrite length_take length_drop Hlen.
         iSplitL; [|iPureIntro; rewrite length_drop; lia]. 
         assert (1 `min` (res - cap - (cap - 1)) = 1); [rewrite min_l; [done|lia]|]. 
@@ -219,28 +222,27 @@ Section Hoare.
       assert (length (drop (cap - 1) vs) > 0); [rewrite length_drop Hlen; lia|].
       destruct (drop (cap - 1) vs); [rewrite length_nil in H4; lia|]. simpl.
       rewrite take_0. iDestruct (array_singleton with "Hun1") as "Hun1".
-      iExists v. iFrame. iSplitR; [by iPureIntro|]. iExists (cap + cap - 1).
-      iSplitL; [|iPureIntro; lia]. 
-      rewrite -Z.add_assoc. 
+      iExists v. iFrame. iSplitR; [by iPureIntro|]. iExists res, (cap + cap - 1). 
+      iFrame "Hal1". iSplitL; [|iPureIntro; lia]. rewrite -Z.add_assoc. 
       assert ((3 + (cap + cap) - 1)%Z = (3 + (cap + cap - 1))%Z) by lia. 
       rewrite H5 Nat2Z.inj_sub; [|lia]. by rewrite Nat2Z.inj_add. }
     wp_pures. destruct (decide (res - cap = 0)) as [Hcr2 | Hcr2]. 
     { rewrite -Nat2Z.inj_sub; [|done]. rewrite Hcr2. wp_pures. 
-      iApply "Hphi". iSplitL; [iFrame; iPureIntro; auto|]. iRight. by iPureIntro. }
+      iApply "Hphi". iSplitL; [iFrame; iFrame "Hal1"; iPureIntro; lia|].
+      iRight. by iPureIntro. }
     case_bool_decide; [inv H1; lia|]. wp_pures.
     iPoseProof (freelist_extend_hoare al al res (al +ₗ (3 + cap)) cap 
     (res - cap - 1) 0 (res - cap - 1)) as "H"; [lia|done|done|lia|]. 
     assert (Z.of_nat (res - cap - 1) = (Z.of_nat res - Z.of_nat cap - 1)%Z) by lia.
-    rewrite H2.  
-    rewrite -(take_drop (res - cap - 1) vs). 
+    rewrite H2 -(take_drop (res - cap - 1) vs). 
     iDestruct (array_app with "Hun") as "(Hun1 & Hun2)".
     wp_apply ("H" with "[Hisfl Hun1]"). 
-    { iFrame "Hisfl". iExists (take (res - cap - 1) vs). iSplitL "Hun1"; [
+    { iFrame "Hal1 Hisfl". iExists (take (res - cap - 1) vs). iSplitL "Hun1"; [
       by rewrite Loc.add_assoc Z.add_0_r|]. iPureIntro. rewrite length_take. lia. }
     iIntros "Hisfl". wp_store. wp_pures. iApply "Hphi".
     rewrite -(take_drop 1 (drop (res - cap - 1) vs)). 
     iDestruct (array_app with "Hun2") as "(Hun1 & Hun2)". iSplitR "Hun1". 
-    { iExists (cap + (res - cap)),  (drop (res - cap) vs). 
+    { iExists res, (cap + (res - cap)),  (drop (res - cap) vs). iFrame "Hal1".
       rewrite -Nat2Z.inj_sub; [|done]. rewrite Nat2Z.inj_add. iFrame.
       iSplitR; [done|]. iSplitR; [iPureIntro; lia|]. rewrite length_take.
       iSplitL; [|iPureIntro; rewrite length_drop Hlen; lia].
@@ -260,28 +262,28 @@ Section Hoare.
     assert ((3 + cap + Z.of_nat (res - cap - 1))%Z = 
     (3 + cap + Z.of_nat (res - cap) - 1)%Z) by lia. 
     rewrite H5. iExists (al +ₗ (3 + cap + (res - cap)%nat - 1)), v. iSplitR; 
-    [by iPureIntro|]. iFrame. iExists (cap + (res - cap)%nat - 1). 
+    [by iPureIntro|]. iFrame. iExists res, (cap + (res - cap)%nat - 1). iFrame "Hal1".
     iSplitR; [iPureIntro|iPureIntro; lia]. 
     rewrite -Z.add_assoc -Nat2Z.inj_add -Z.add_sub_assoc Nat2Z.inj_sub; [done|lia].
   Qed.
 
-  Lemma alloc_hoare al res :
-    {{{ is_allocator al res }}}
+  Lemma alloc_hoare al :
+    {{{ is_allocator al }}}
       alloc #al
-    {{{ vret, RET vret; is_allocator al res ∗
-      ((∃ l v, ⌜vret = SOMEV #l⌝ ∗ l ↦ v ∗ is_valid_loc l al res)
+    {{{ vret, RET vret; 
+      is_allocator al ∗
+      ((∃ l v, ⌜vret = SOMEV #l⌝ ∗ l ↦ v ∗ is_valid_loc l al)
         ∨ 
       ⌜vret = NONEV⌝)
     }}}.
   Proof.
-    iIntros (φ) "(%cap & %vs & %Hr & %Hcr & Hal1 & Hal2 & Hisfl & Hun & %Hlen) Hphi". 
+    iIntros (φ) "(%res&%cap&%vs&%Hr& %Hcr & Hal1 & Hal2 & Hisfl & Hun & %Hlen) Hphi". 
     iUnfold alloc. wp_pures. wp_apply (freelist_pop_hoare with "Hisfl"). 
-    iIntros (v) "[(-> & Hisfl)|(%l & %v' & -> & Hl & #Hlv & Hisfl)]".
+    iIntros (v) "(Hisfl & [->|(%l & %v' & -> & Hl & #Hlv)])".
     { wp_pures. wp_apply (extend_hoare with "[Hal1 Hal2 Hun Hisfl]"); 
-      [iExists cap, vs; iFrame; iPureIntro; lia|]. 
-      iIntros (v) "(Hal & [(%l & %v' & -> & Hisfl)| ->])"; 
+      [iFrame; iPureIntro; lia|]. iIntros (v) "(Hal & [(%l & %v' & -> & Hisfl)| ->])"; 
       iApply "Hphi"; iSplitL "Hal"; try done; [iLeft; by iFrame|by iRight]. }
-    wp_pures. iApply "Hphi". iSplitR "Hl"; [iExists cap, vs; iFrame; iPureIntro; lia|].
+    wp_pures. iApply "Hphi". iSplitR "Hl"; [iFrame; iPureIntro; lia|].
     iLeft. iFrame. iSplitR; [by iPureIntro|done]. 
   Qed.
 
